src/riot/asn1/ASN1.Spec.TLV.fst
@@ -9,6 +9,8 @@ open ASN1.Spec.Value.BOOLEAN
 open ASN1.Spec.Value.NULL
 open ASN1.Spec.Value.INTEGER
 open ASN1.Spec.Value.OCTET_STRING
+open ASN1.Spec.Value.IA5_STRING
+open ASN1.Spec.Value.PRINTABLE_STRING
 open ASN1.Spec.Value.BIT_STRING
 open ASN1.Spec.Value.OID
 open ASN1.Spec.Value.SEQUENCE
@@ -18,7 +20,7 @@ open FStar.Integers
 
 (* NOTE: Read after `ASN1.Spec.Tag`, `ASN1.Spec.Length`, `ASN1.Spec.Value.*` *)
 
-/// Interfaces to make this library easier to use, WIP
+/// Interfaces to make this library easier to use
 ///
 inline_for_extraction noextract
 let parse_asn1_TLV_kind_of_type
@@ -26,9 +28,12 @@ let parse_asn1_TLV_kind_of_type
 : parser_kind
 = match _a with
   | BOOLEAN      -> parse_asn1_boolean_TLV_kind
-  | ASN1_NULL         -> parse_asn1_ASN1_NULL_TLV_kind
+  | ASN1_NULL    -> parse_asn1_ASN1_NULL_TLV_kind
   | INTEGER      -> parse_asn1_integer_TLV_kind
   | OCTET_STRING -> parse_asn1_octet_string_TLV_kind
+  | PRINTABLE_STRING
+                 -> parse_asn1_printable_string_TLV_kind
+  | IA5_STRING   -> parse_asn1_ia5_string_TLV_kind
   | BIT_STRING   -> parse_asn1_bit_string_TLV_kind
   | OID          -> parse_asn1_oid_TLV_kind
 
@@ -38,9 +43,12 @@ let parse_asn1_TLV_of_type
 : parser (parse_asn1_TLV_kind_of_type _a) (datatype_of_asn1_type _a)
 = match _a with
   | BOOLEAN      -> parse_asn1_boolean_TLV
-  | ASN1_NULL         -> parse_asn1_ASN1_NULL_TLV
+  | ASN1_NULL    -> parse_asn1_ASN1_NULL_TLV
   | INTEGER      -> parse_asn1_integer_TLV
   | OCTET_STRING -> parse_asn1_octet_string_TLV
+  | PRINTABLE_STRING
+                 -> parse_asn1_printable_string_TLV
+  | IA5_STRING   -> parse_asn1_ia5_string_TLV
   | BIT_STRING   -> parse_asn1_bit_string_TLV
   | OID          -> parse_asn1_oid_TLV
 
@@ -50,9 +58,12 @@ let serialize_asn1_TLV_of_type
 : serializer (parse_asn1_TLV_of_type _a)
 = match _a with
   | BOOLEAN      -> serialize_asn1_boolean_TLV
-  | ASN1_NULL         -> serialize_asn1_ASN1_NULL_TLV
+  | ASN1_NULL    -> serialize_asn1_ASN1_NULL_TLV
   | INTEGER      -> serialize_asn1_integer_TLV
   | OCTET_STRING -> serialize_asn1_octet_string_TLV
+  | PRINTABLE_STRING
+                 -> serialize_asn1_printable_string_TLV
+  | IA5_STRING   -> serialize_asn1_ia5_string_TLV
   | BIT_STRING   -> serialize_asn1_bit_string_TLV
   | OID          -> serialize_asn1_oid_TLV
 
@@ -67,9 +78,12 @@ let length_of_asn1_primitive_value
   length == Seq.length (
     match _a with
     | BOOLEAN      -> serialize serialize_asn1_boolean value
-    | ASN1_NULL         -> serialize serialize_asn1_ASN1_NULL value
+    | ASN1_NULL    -> serialize serialize_asn1_ASN1_NULL value
     | INTEGER      -> serialize (serialize_asn1_integer (length_of_asn1_integer (value <: datatype_of_asn1_type INTEGER))) value
     | OCTET_STRING -> serialize (serialize_asn1_octet_string (v (dfst (value <: datatype_of_asn1_type OCTET_STRING)))) value
+    | PRINTABLE_STRING
+                   -> serialize (serialize_asn1_printable_string (dfst (value <: datatype_of_asn1_type PRINTABLE_STRING))) value
+    | IA5_STRING   -> serialize (serialize_asn1_ia5_string (dfst (value <: datatype_of_asn1_type IA5_STRING))) value
     | BIT_STRING   -> serialize (serialize_asn1_bit_string (v (Mkbit_string_t?.bs_len (value <: datatype_of_asn1_type BIT_STRING)))) value
     | OID          -> serialize (serialize_asn1_oid (length_of_oid (value <: datatype_of_asn1_type OID))) value )
   })
@@ -92,6 +106,17 @@ let length_of_asn1_primitive_value
                       lemma_serialize_asn1_octet_string_size length value
                     ; length )
 
+  | PRINTABLE_STRING
+                 -> ( let value = value <: datatype_of_asn1_type PRINTABLE_STRING in
+                      let length = v (dfst value) in
+                      lemma_serialize_asn1_printable_string_size (dfst value) value
+                    ; length )
+
+  | IA5_STRING   -> ( let value = value <: datatype_of_asn1_type IA5_STRING in
+                      let length = v (dfst value) in
+                      lemma_serialize_asn1_ia5_string_size (dfst value) value
+                    ; length )
+
   | BIT_STRING   -> ( let value = value <: datatype_of_asn1_type BIT_STRING in
                       let length = v (Mkbit_string_t?.bs_len value) in
                       lemma_serialize_asn1_bit_string_size length value
@@ -105,7 +130,8 @@ let length_of_asn1_primitive_value
 
 /// Length Spec of ASN.1 Primitive [TAG, LEN, VALUE] of primitive types
 ///
-#push-options "--z3rlimit 32"
+#restart-solver
+#push-options "--z3rlimit 32 --fuel 2 --ifuel 1"
 noextract
 let length_of_asn1_primitive_TLV
   (#_a: asn1_primitive_type)
@@ -117,7 +143,7 @@ let length_of_asn1_primitive_TLV
                 | BOOLEAN      -> ( let value = value <: datatype_of_asn1_type BOOLEAN in
                                     lemma_serialize_asn1_boolean_TLV_size value )
 
-                | ASN1_NULL         -> ( let value = value <: datatype_of_asn1_type ASN1_NULL in
+                | ASN1_NULL    -> ( let value = value <: datatype_of_asn1_type ASN1_NULL in
                                     lemma_serialize_asn1_ASN1_NULL_TLV_size value )
 
                 | INTEGER      -> ( let value = value <: datatype_of_asn1_type INTEGER in
@@ -129,6 +155,12 @@ let length_of_asn1_primitive_TLV
                                     let length = v (dfst value) in
                                     let len: asn1_value_int32_of_type OCTET_STRING = u length in
                                     lemma_serialize_asn1_octet_string_TLV_size value )
+
+                | PRINTABLE_STRING
+                               -> ( lemma_serialize_asn1_printable_string_TLV_size (value <: datatype_of_asn1_type PRINTABLE_STRING) )
+
+                | IA5_STRING   -> ( let value = value <: datatype_of_asn1_type IA5_STRING in
+                                    lemma_serialize_asn1_ia5_string_TLV_size value )
 
                 | BIT_STRING   -> ( let value = value <: datatype_of_asn1_type BIT_STRING in
                                     let length = v (Mkbit_string_t?.bs_len value) in
@@ -159,6 +191,19 @@ let length_of_asn1_primitive_TLV
                       let length = v (dfst value) in
                       let len: asn1_value_int32_of_type OCTET_STRING = u length in
                       lemma_serialize_asn1_octet_string_TLV_size value
+                    ; 1 + length_of_asn1_length len + length )
+
+  | PRINTABLE_STRING
+                 -> ( let value = value <: datatype_of_asn1_type PRINTABLE_STRING in
+                      let len: asn1_value_int32_of_type PRINTABLE_STRING = dfst value in
+                      let length: asn1_value_length_of_type PRINTABLE_STRING = v len in
+                      lemma_serialize_asn1_printable_string_TLV_size value
+                    ; 1 + length_of_asn1_length len + length )
+
+  | IA5_STRING   -> ( let value = value <: datatype_of_asn1_type IA5_STRING in
+                      let len: asn1_value_int32_of_type IA5_STRING = dfst value in
+                      let length: asn1_value_length_of_type IA5_STRING = v len in
+                      lemma_serialize_asn1_ia5_string_TLV_size value
                     ; 1 + length_of_asn1_length len + length )
 
   | BIT_STRING   -> ( let value = value <: datatype_of_asn1_type BIT_STRING in
