src/riot/asn1/ASN1.Low.TLV.fst
@@ -8,6 +8,8 @@ open ASN1.Spec.Value.BOOLEAN
 open ASN1.Spec.Value.NULL
 open ASN1.Spec.Value.INTEGER
 open ASN1.Spec.Value.OCTET_STRING
+open ASN1.Spec.Value.IA5_STRING
+open ASN1.Spec.Value.PRINTABLE_STRING
 open ASN1.Spec.Value.BIT_STRING
 open ASN1.Spec.Value.OID
 open ASN1.Spec.Value.SEQUENCE
@@ -23,6 +25,8 @@ open ASN1.Low.Value.BOOLEAN
 open ASN1.Low.Value.NULL
 open ASN1.Low.Value.INTEGER
 open ASN1.Low.Value.OCTET_STRING
+open ASN1.Low.Value.IA5_STRING
+open ASN1.Low.Value.PRINTABLE_STRING
 open ASN1.Low.Value.BIT_STRING
 open ASN1.Low.Value.OID
 open ASN1.Low.Value.SEQUENCE
@@ -50,12 +54,19 @@ let len_of_asn1_primitive_value
 = match _a with
   | BOOLEAN      -> ( 1ul )
 
-  | ASN1_NULL         -> ( 0ul )
+  | ASN1_NULL    -> ( 0ul )
 
   | INTEGER      -> ( let value = value <: datatype_of_asn1_type INTEGER in
                       len_of_asn1_integer value )
 
   | OCTET_STRING -> ( let value = value <: datatype_of_asn1_type OCTET_STRING in
+                      dfst value )
+
+  | PRINTABLE_STRING
+                 -> ( let value = value <: datatype_of_asn1_type PRINTABLE_STRING in
+                      dfst value )
+
+  | IA5_STRING   -> ( let value = value <: datatype_of_asn1_type IA5_STRING in
                       dfst value )
 
   | BIT_STRING   -> ( let value = value <: datatype_of_asn1_type BIT_STRING in
@@ -65,7 +76,8 @@ let len_of_asn1_primitive_value
                       len_of_oid_buffer value )
 #pop-options
 
-#push-options "--z3rlimit 64"
+#restart-solver
+#push-options "--z3rlimit 128 --fuel 2 --ifuel 1"
 inline_for_extraction noextract
 let len_of_asn1_primitive_TLV
   (#_a: asn1_primitive_type)
@@ -74,12 +86,17 @@ let len_of_asn1_primitive_TLV
 = (* Prf *) ( match _a with
               | BOOLEAN      -> ( lemma_serialize_asn1_boolean_TLV_size        (value <: datatype_of_asn1_type BOOLEAN     )
                                 ; lemma_serialize_asn1_boolean_TLV_unfold      (value <: datatype_of_asn1_type BOOLEAN     ) )
-              | ASN1_NULL         -> ( lemma_serialize_asn1_ASN1_NULL_TLV_size           (value <: datatype_of_asn1_type ASN1_NULL        )
-                                ; lemma_serialize_asn1_ASN1_NULL_TLV_unfold         (value <: datatype_of_asn1_type ASN1_NULL        ) )
+              | ASN1_NULL    -> ( lemma_serialize_asn1_ASN1_NULL_TLV_size      (value <: datatype_of_asn1_type ASN1_NULL   )
+                                ; lemma_serialize_asn1_ASN1_NULL_TLV_unfold    (value <: datatype_of_asn1_type ASN1_NULL   ) )
               | INTEGER      -> ( lemma_serialize_asn1_integer_TLV_size        (value <: datatype_of_asn1_type INTEGER     )
                                 ; lemma_serialize_asn1_integer_TLV_unfold      (value <: datatype_of_asn1_type INTEGER     ) )
               | OCTET_STRING -> ( lemma_serialize_asn1_octet_string_TLV_size   (value <: datatype_of_asn1_type OCTET_STRING)
                                 ; lemma_serialize_asn1_octet_string_TLV_unfold (value <: datatype_of_asn1_type OCTET_STRING) )
+              | PRINTABLE_STRING
+                             -> ( lemma_serialize_asn1_printable_string_TLV_size   (value <: datatype_of_asn1_type PRINTABLE_STRING  )
+                                ; lemma_serialize_asn1_printable_string_TLV_unfold (value <: datatype_of_asn1_type PRINTABLE_STRING  ) )
+              | IA5_STRING   -> ( lemma_serialize_asn1_ia5_string_TLV_size     (value <: datatype_of_asn1_type IA5_STRING  )
+                                ; lemma_serialize_asn1_ia5_string_TLV_unfold   (value <: datatype_of_asn1_type IA5_STRING  ) )
               | BIT_STRING   -> ( lemma_serialize_asn1_bit_string_TLV_size     (value <: datatype_of_asn1_type BIT_STRING  )
                                 ; lemma_serialize_asn1_bit_string_TLV_unfold   (value <: datatype_of_asn1_type BIT_STRING  ) )
               | OID          -> ( lemma_serialize_asn1_oid_TLV_size            (value <: datatype_of_asn1_type OID         )
@@ -102,9 +119,12 @@ let serialize32_asn1_TLV_backwards_of_type
 : serializer32_backwards (serialize_asn1_TLV_of_type _a)
 = match _a with
   | BOOLEAN      -> serialize32_asn1_boolean_TLV_backwards      ()
-  | ASN1_NULL         -> serialize32_asn1_ASN1_NULL_TLV_backwards         ()
+  | ASN1_NULL    -> serialize32_asn1_ASN1_NULL_TLV_backwards    ()
   | INTEGER      -> serialize32_asn1_integer_TLV_backwards      ()
   | OCTET_STRING -> serialize32_asn1_octet_string_TLV_backwards ()
+  | PRINTABLE_STRING
+                 -> serialize32_asn1_printable_string_TLV_backwards
+  | IA5_STRING   -> serialize32_asn1_ia5_string_TLV_backwards
   | BIT_STRING   -> serialize32_asn1_bit_string_TLV_backwards   ()
   | OID          -> serialize32_asn1_oid_TLV_backwards          ()
 
