src/riot/asn1/ASN1.Low.Value.StringTypes.fst
@@ -70,7 +70,6 @@ let serialize32_asn1_string_TLV_backwards
                                  { x == synth_string len s32 }))
   (prf: unit { forall len. synth_injective (synth_string len) })
 : serializer32_backwards (serialize_asn1_string_TLV t len_of_string filter_string synth_string synth_string_inverse prf)
-// : serializer (parse_asn1_string_TLV t len_of_string filter_string synth_string prf)
 = serialize32_tagged_union_backwards
   (* lst*) (serialize32_asn1_tag_of_type_backwards t
             `serialize32_nondep_then_backwards`
@@ -85,3 +84,26 @@ let serialize32_asn1_string_TLV_backwards
                     (* g1'*) (synth_asn1_string_V_inverse t len_of_string x)
                     (* prf*) ()))
 
+
+let serialize32_asn1_string_TLV_with_character_bound_backwards
+  (t: asn1_type { t == IA5_STRING \/ t == PRINTABLE_STRING \/ t == OCTET_STRING })
+  (len_of_string: datatype_of_asn1_type t -> asn1_value_int32_of_type t)
+  (filter_string: (len: asn1_value_int32_of_type t)
+                  -> (s32: B32.lbytes32 len)
+                  -> GTot (bool))
+  (synth_string: (len: asn1_value_int32_of_type t)
+                       -> (s32: parse_filter_refine (filter_string len))
+                       -> GTot (x: datatype_of_asn1_type t
+                                  { len_of_string x== len }))
+  (synth_string_inverse: (len: asn1_value_int32_of_type t)
+                         -> (x: datatype_of_asn1_type t { len_of_string x== len })
+                         -> (s32: parse_filter_refine (filter_string len)
+                                 { x == synth_string len s32 }))
+  (prf: unit { forall len. synth_injective (synth_string len) })
+  (count_character: (x: datatype_of_asn1_type t) -> Tot (asn1_int32))
+  (lb: asn1_int32)
+  (ub: asn1_int32 { lb <= ub })
+: serializer32_backwards (serialize_asn1_string_TLV_with_character_bound t len_of_string filter_string synth_string synth_string_inverse prf count_character lb ub)
+= serialize32_asn1_string_TLV_backwards t len_of_string filter_string synth_string synth_string_inverse prf
+  `serialize32_filter_backwards`
+  filter_asn1_string_with_character_bound t count_character lb ub
