src/riot/asn1/ASN1.Spec.Value.IA5_STRING.fst
@@ -1,0 +1,140 @@
+module ASN1.Spec.Value.IA5_STRING
+
+open ASN1.Spec.Base
+open LowParse.Spec.Bytes
+
+open ASN1.Base
+open ASN1.Spec.Tag
+open ASN1.Spec.Length
+open ASN1.Spec.Value.StringTypes
+
+open FStar.Integers
+
+module B32 = FStar.Bytes
+
+let filter_asn1_ia5_string
+  (len: asn1_value_int32_of_type IA5_STRING)
+  (s32: B32.lbytes32 len)
+: GTot (bool)
+= let s = B32.reveal s32 in
+  Seq.for_all valid_IA5_byte s
+
+let synth_asn1_ia5_string
+  (len: asn1_value_int32_of_type IA5_STRING)
+  (s32: parse_filter_refine (filter_asn1_ia5_string len))
+: GTot (value: datatype_of_asn1_type IA5_STRING{(dfst value) == len})
+= (|len, s32|)
+
+let synth_asn1_ia5_string_inverse
+  (len: asn1_value_int32_of_type IA5_STRING)
+  (value: datatype_of_asn1_type IA5_STRING{(dfst value) == len})
+: Tot (s32: parse_filter_refine (filter_asn1_ia5_string len)
+             { value == synth_asn1_ia5_string len s32 })
+= dsnd value
+
+let parse_asn1_ia5_string
+= parse_asn1_string
+    (IA5_STRING)
+    (dfst)
+    (filter_asn1_ia5_string)
+    (synth_asn1_ia5_string)
+    ()
+
+let serialize_asn1_ia5_string
+= serialize_asn1_string
+    (IA5_STRING)
+    (dfst)
+    (filter_asn1_ia5_string)
+    (synth_asn1_ia5_string)
+    (synth_asn1_ia5_string_inverse)
+    ()
+
+let lemma_serialize_asn1_ia5_string_unfold
+= lemma_serialize_asn1_string_unfold
+    (IA5_STRING)
+    (dfst)
+    (filter_asn1_ia5_string)
+    (synth_asn1_ia5_string)
+    (synth_asn1_ia5_string_inverse)
+    ()
+
+let lemma_serialize_asn1_ia5_string_size
+= lemma_serialize_asn1_string_size
+    (IA5_STRING)
+    (dfst)
+    (filter_asn1_ia5_string)
+    (synth_asn1_ia5_string)
+    (synth_asn1_ia5_string_inverse)
+    ()
+
+let parse_asn1_ia5_string_TLV_kind = parse_asn1_string_TLV_kind IA5_STRING
+let parse_asn1_ia5_string_TLV
+: parser parse_asn1_ia5_string_TLV_kind (datatype_of_asn1_type IA5_STRING)
+= parse_asn1_string_TLV
+    (IA5_STRING)
+    (dfst)
+    (filter_asn1_ia5_string)
+    (synth_asn1_ia5_string)
+    ()
+
+let serialize_asn1_ia5_string_TLV
+: serializer (parse_asn1_ia5_string_TLV)
+= serialize_asn1_string_TLV
+    (IA5_STRING)
+    (dfst)
+    (filter_asn1_ia5_string)
+    (synth_asn1_ia5_string)
+    (synth_asn1_ia5_string_inverse)
+    ()
+
+let lemma_serialize_asn1_ia5_string_TLV_unfold
+= lemma_serialize_asn1_string_TLV_unfold
+    (IA5_STRING)
+    (dfst)
+    (filter_asn1_ia5_string)
+    (synth_asn1_ia5_string)
+    (synth_asn1_ia5_string_inverse)
+    ()
+
+let lemma_serialize_asn1_ia5_string_TLV_size
+= lemma_serialize_asn1_string_TLV_size
+    (IA5_STRING)
+    (dfst)
+    (filter_asn1_ia5_string)
+    (synth_asn1_ia5_string)
+    (synth_asn1_ia5_string_inverse)
+    ()
+
+let count_ia5_character
+  (x: datatype_of_asn1_type IA5_STRING)
+: Tot (asn1_int32)
+= dfst x
+
+let parse_asn1_ia5_string_TLV_with_character_bound
+  (lb: asn1_int32)
+  (ub: asn1_int32 { lb <= ub })
+: parser parse_asn1_ia5_string_TLV_kind (asn1_string_with_character_bound_t IA5_STRING count_ia5_character lb ub)
+= parse_asn1_string_TLV_with_character_bound
+    (IA5_STRING)
+    (dfst)
+    (filter_asn1_ia5_string)
+    (synth_asn1_ia5_string)
+    ()
+    (count_ia5_character)
+    (lb)
+    (ub)
+
+let serialize_asn1_ia5_string_TLV_with_character_bound
+  (lb: asn1_int32)
+  (ub: asn1_int32 { lb <= ub })
+: serializer (parse_asn1_ia5_string_TLV_with_character_bound lb ub)
+= serialize_asn1_string_TLV_with_character_bound
+    (IA5_STRING)
+    (dfst)
+    (filter_asn1_ia5_string)
+    (synth_asn1_ia5_string)
+    (synth_asn1_ia5_string_inverse)
+    ()
+    (count_ia5_character)
+    (lb)
+    (ub)
